passing coq 8.2 -> 8.4

Coccinelle/examples/cime_trace/Newman.v.d
@@ -1,1 +1,0 @@
-examples/cime_trace/Newman.vo examples/cime_trace/Newman.glob: examples/cime_trace/Newman.v list_extensions/weaved_relation.vo basis/closure.vo basis/terminaison.vo term_algebra/equational_theory_spec.vo
