Coccinelle/examples/cime_trace/arith_extension.v.d
@@ -1,1 +1,0 @@
-examples/cime_trace/arith_extension.vo examples/cime_trace/arith_extension.glob: examples/cime_trace/arith_extension.v
