Coccinelle/examples/cime_trace/rewriting.v.d
@@ -1,1 +1,0 @@
-examples/cime_trace/rewriting.vo examples/cime_trace/rewriting.glob: examples/cime_trace/rewriting.v term_algebra/term.vo term_algebra/equational_theory.vo
