Coccinelle/examples/cime_trace/term_extension.v.d
@@ -1,1 +1,0 @@
-examples/cime_trace/term_extension.vo examples/cime_trace/term_extension.glob: examples/cime_trace/term_extension.v basis/TransClosure.vo term_algebra/term.vo basis/terminaison.vo
