Coccinelle/basis/decidable_set.v
@@ -17,7 +17,6 @@ Require Import Arith.
 
 Module Type S.
 
-
 Parameter A : Set.
 Parameter eq_bool : A -> A -> bool.
 Parameter eq_bool_ok : forall a1 a2, match eq_bool a1 a2 with true => a1 = a2 | false => ~ a1 = a2 end.
